remove IteratorCollect

src/Init/Data/Iterators/Consumers/Monadic/Collect.lean
@@ -22,41 +22,10 @@ Concretely, the following operations are provided:
 * `IterM.toList`, collecting the values in a list
 * `IterM.toListRev`, collecting the values in a list in reverse order but more efficiently
 * `IterM.toArray`, collecting the values in an array
-
-Some producers and combinators provide specialized implementations. These are captured by the
-`IteratorCollect` type class. They should be implemented by all types of iterators. A default
-implementation is provided. The typeclass `LawfulIteratorCollect` asserts that an `IteratorCollect`
-instance equals the default implementation.
 -/
 
 namespace Std
 open Std.Internal Std.Iterators
-
-section Typeclasses
-
-/--
-`IteratorCollect α m` provides efficient implementations of collectors for `α`-based
-iterators. Right now, it is limited to a potentially optimized `toArray` implementation.
-
-This class is experimental and users of the iterator API should not explicitly depend on it.
-They can, however, assume that consumers that require an instance will work for all iterators
-provided by the standard library.
-
-Note: For this to be compositional enough to be useful, `toArrayMapped` would need to accept a
-termination proof for the specific mapping function used instead of the blanket `Finite α m`
-instance. Otherwise, most combinators like `map` cannot implement their own instance relying on
-the instance of their base iterators. However, fixing this is currently low priority.
--/
-class IteratorCollect (α : Type w) (m : Type w → Type w') (n : Type w → Type w'')
-    {β : Type w} [Iterator α m β] where
-  /--
-  Maps the emitted values of an iterator using the given function and collects the results in an
-  `Array`. This is an internal implementation detail. Consider using `it.map f |>.toArray` instead.
-  -/
-  toArrayMapped :
-    (lift : ⦃δ : Type w⦄ → m δ → n δ) → {γ : Type w} → (β → n γ) → IterM (α := α) m β → n (Array γ)
-
-end Typeclasses
 
 section ToArray
 
@@ -66,7 +35,7 @@ def IterM.DefaultConsumers.toArrayMapped.RecursionRel {α β : Type w} {m : Type
     (x.1.IsPlausibleStep (.skip x'.1) ∧ x'.2 = x.2)
 
 /--
-This is an internal function used in `IteratorCollect.defaultImplementation`.
+This is an internal function used in `IteratorCollect.defaultImplementation`. -- TODO
 
 It iterates over an iterator and applies `f` whenever a value is emitted before inserting the result
 of `f` into an array.
@@ -91,45 +60,6 @@ where
       | .done _ => return acc) it acc
 
 /--
-This is the default implementation of the `IteratorCollect` class.
-It simply iterates through the iterator using `IterM.step`, incrementally building up the desired
-data structure. For certain iterators, more efficient implementations are possible and should be
-used instead.
--/
-@[always_inline]
-def IteratorCollect.defaultImplementation {α β : Type w} {m : Type w → Type w'}
-    {n : Type w → Type w''} [Monad n] [Iterator α m β] :
-    IteratorCollect α m n where
-  toArrayMapped := IterM.DefaultConsumers.toArrayMapped
-
-/--
-Asserts that a given `IteratorCollect` instance is equal to `IteratorCollect.defaultImplementation`
-*if the underlying iterator is finite*.
-(Even though equal, the given instance might be vastly more efficient.)
--/
-class LawfulIteratorCollect (α : Type w) (m : Type w → Type w') (n : Type w → Type w'')
-    {β : Type w} [Monad m] [Monad n] [Iterator α m β] [i : IteratorCollect α m n] where
-  lawful_toArrayMapped : ∀ lift [LawfulMonadLiftFunction lift] [Finite α m],
-    i.toArrayMapped lift (α := α) (γ := γ)
-      = IteratorCollect.defaultImplementation.toArrayMapped lift
-
-theorem LawfulIteratorCollect.toArrayMapped_eq {α β γ : Type w} {m : Type w → Type w'}
-    {n : Type w → Type w''} [Monad m] [Monad n] [Iterator α m β] [Finite α m] [IteratorCollect α m n]
-    [hl : LawfulIteratorCollect α m n] {lift : ⦃δ : Type w⦄ → m δ → n δ}
-    [LawfulMonadLiftFunction lift]
-    {f : β → n γ} {it : IterM (α := α) m β} :
-    IteratorCollect.toArrayMapped lift f it (m := m) =
-      IterM.DefaultConsumers.toArrayMapped lift f it (m := m) := by
-  rw [lawful_toArrayMapped]; rfl
-
-instance instLawfulIteratorCollectDefaultImplementation (α β : Type w) (m : Type w → Type w')
-    (n : Type w → Type w'') [Monad n] [Iterator α m β] [Monad m] [Iterator α m β] [Finite α m] :
-    haveI : IteratorCollect α m n := .defaultImplementation
-    LawfulIteratorCollect α m n :=
-  letI : IteratorCollect α m n := .defaultImplementation
-  ⟨fun _ => rfl⟩
-
-/--
 Traverses the given iterator and stores the emitted values in an array.
 
 If the iterator is not finite, this function might run forever. The variant
@@ -137,8 +67,8 @@ If the iterator is not finite, this function might run forever. The variant
 -/
 @[always_inline, inline]
 def IterM.toArray {α β : Type w} {m : Type w → Type w'} [Monad m] [Iterator α m β]
-    [IteratorCollect α m m] (it : IterM (α := α) m β) : m (Array β) :=
-  IteratorCollect.toArrayMapped (fun ⦃_⦄ => id) pure it
+    (it : IterM (α := α) m β) : m (Array β) :=
+  DefaultConsumers.toArrayMapped (fun ⦃_⦄ => id) pure it
 
 /--
 Traverses the given iterator and stores the emitted values in an array.
@@ -147,7 +77,7 @@ This function is deprecated. Instead of `it.allowNontermination.toArray`, use `i
 -/
 @[always_inline, inline, deprecated IterM.toArray (since := "2025-10-23")]
 def IterM.Partial.toArray {α : Type w} {m : Type w → Type w'} {β : Type w} [Monad m]
-    [Iterator α m β] (it : IterM.Partial (α := α) m β) [IteratorCollect α m m] : m (Array β) :=
+    [Iterator α m β] (it : IterM.Partial (α := α) m β) : m (Array β) :=
   it.it.toArray
 
 /--
@@ -158,7 +88,7 @@ finite. If such a proof is not available, consider using `IterM.toArray`.
 -/
 @[always_inline, inline]
 def IterM.Total.toArray {α : Type w} {m : Type w → Type w'} {β : Type w} [Monad m]
-    [Iterator α m β] [Finite α m] (it : IterM.Total (α := α) m β) [IteratorCollect α m m] :
+    [Iterator α m β] [Finite α m] (it : IterM.Total (α := α) m β) :
     m (Array β) :=
   it.it.toArray
 
@@ -218,7 +148,7 @@ If the iterator is not finite, this function might run forever. The variant
 -/
 @[always_inline, inline]
 def IterM.toList {α : Type w} {m : Type w → Type w'} [Monad m] {β : Type w}
-    [Iterator α m β] [IteratorCollect α m m] (it : IterM (α := α) m β) : m (List β) :=
+    [Iterator α m β] (it : IterM (α := α) m β) : m (List β) :=
   Array.toList <$> IterM.toArray it
 
 /--
@@ -229,7 +159,7 @@ This function is deprecated. Instead of `it.allowNontermination.toList`, use `it
 -/
 @[always_inline, inline, deprecated IterM.toList (since := "2025-10-23")]
 def IterM.Partial.toList {α : Type w} {m : Type w → Type w'} [Monad m] {β : Type w}
-    [Iterator α m β] (it : IterM.Partial (α := α) m β) [IteratorCollect α m m] :
+    [Iterator α m β] (it : IterM.Partial (α := α) m β) :
     m (List β) :=
   Array.toList <$> it.it.toArray
 
@@ -242,7 +172,7 @@ finite. If such a proof is not available, consider using `IterM.toList`.
 -/
 @[always_inline, inline]
 def IterM.Total.toList {α : Type w} {m : Type w → Type w'} {β : Type w} [Monad m]
-    [Iterator α m β] [Finite α m] (it : IterM.Total (α := α) m β) [IteratorCollect α m m] :
+    [Iterator α m β] [Finite α m] (it : IterM.Total (α := α) m β) :
     m (List β) :=
   it.it.toList
 
