src/Init/Data/Iterators/Lemmas/Combinators/Monadic/Attach.lean
@@ -26,8 +26,7 @@ theorem IterM.step_attachWith [Iterator α m β] [Monad m] {it : IterM (α := α
 @[simp]
 theorem IterM.map_unattach_toList_attachWith [Iterator α m β] [Monad m]
     {it : IterM (α := α) m β} {hP}
-    [Finite α m] [IteratorCollect α m m]
-    [LawfulMonad m] [LawfulIteratorCollect α m m] :
+    [Finite α m] [LawfulMonad m] :
     List.unattach <$> (it.attachWith P hP).toList = it.toList := by
   induction it using IterM.inductSteps with | step it ihy ihs
   rw [IterM.toList_eq_match_step, IterM.toList_eq_match_step, step_attachWith]
@@ -46,8 +45,7 @@ theorem IterM.map_unattach_toList_attachWith [Iterator α m β] [Monad m]
 @[simp]
 theorem IterM.map_unattach_toListRev_attachWith [Iterator α m β] [Monad m] [Monad n]
     {it : IterM (α := α) m β} {hP}
-    [Finite α m] [IteratorCollect α m m]
-    [LawfulMonad m] [LawfulIteratorCollect α m m] :
+    [Finite α m] [LawfulMonad m] :
     List.unattach <$> (it.attachWith P hP).toListRev = it.toListRev := by
   rw [toListRev_eq, toListRev_eq, ← map_unattach_toList_attachWith (it := it) (hP := hP)]
   simp [-map_unattach_toList_attachWith]
@@ -55,8 +53,8 @@ theorem IterM.map_unattach_toListRev_attachWith [Iterator α m β] [Monad m] [Mo
 @[simp]
 theorem IterM.map_unattach_toArray_attachWith [Iterator α m β] [Monad m] [Monad n]
     {it : IterM (α := α) m β} {hP}
-    [Finite α m] [IteratorCollect α m m]
-    [LawfulMonad m] [LawfulIteratorCollect α m m] :
+    [Finite α m]
+    [LawfulMonad m] :
     (·.map Subtype.val) <$> (it.attachWith P hP).toArray = it.toArray := by
   rw [← toArray_toList, ← toArray_toList, ← map_unattach_toList_attachWith (it := it) (hP := hP)]
   simp [-map_unattach_toList_attachWith, -IterM.toArray_toList]
@@ -66,7 +64,6 @@ theorem IterM.count_attachWith [Iterator α m β] [Monad m] [Monad n]
     {it : IterM (α := α) m β} {hP}
     [Finite α m] [IteratorLoop α m m] [LawfulMonad m] [LawfulIteratorLoop α m m] :
     (it.attachWith P hP).count = it.count := by
-  letI : IteratorCollect α m m := .defaultImplementation
   rw [← up_length_toList_eq_count, ← up_length_toList_eq_count,
     ← map_unattach_toList_attachWith (it := it) (P := P) (hP := hP)]
   simp only [Functor.map_map, List.length_unattach]
