src/Init/Data/Iterators/Lemmas/Combinators/Monadic/ULift.lean
@@ -31,8 +31,8 @@ theorem IterM.step_uLift [Iterator α m β] [Monad n] {it : IterM (α := α) m �
 
 @[simp]
 theorem IterM.toList_uLift [Iterator α m β] [Monad m] [Monad n] {it : IterM (α := α) m β}
-    [MonadLiftT m (ULiftT n)] [Finite α m] [IteratorCollect α m m]
-    [LawfulMonad m] [LawfulMonad n] [LawfulIteratorCollect α m m]
+    [MonadLiftT m (ULiftT n)] [Finite α m]
+    [LawfulMonad m] [LawfulMonad n]
     [LawfulMonadLiftT m (ULiftT n)] :
     (it.uLift n).toList =
       (fun l => l.down.map ULift.up) <$> (monadLift it.toList : ULiftT n _).run := by
@@ -47,8 +47,8 @@ theorem IterM.toList_uLift [Iterator α m β] [Monad m] [Monad n] {it : IterM (�
 
 @[simp]
 theorem IterM.toListRev_uLift [Iterator α m β] [Monad m] [Monad n] {it : IterM (α := α) m β}
-    [MonadLiftT m (ULiftT n)] [Finite α m] [IteratorCollect α m m]
-    [LawfulMonad m] [LawfulMonad n] [LawfulIteratorCollect α m m]
+    [MonadLiftT m (ULiftT n)] [Finite α m]
+    [LawfulMonad m] [LawfulMonad n]
     [LawfulMonadLiftT m (ULiftT n)] :
     (it.uLift n).toListRev =
       (fun l => l.down.map ULift.up) <$> (monadLift it.toListRev : ULiftT n _).run := by
@@ -57,8 +57,8 @@ theorem IterM.toListRev_uLift [Iterator α m β] [Monad m] [Monad n] {it : IterM
 
 @[simp]
 theorem IterM.toArray_uLift [Iterator α m β] [Monad m] [Monad n] {it : IterM (α := α) m β}
-    [MonadLiftT m (ULiftT n)] [Finite α m] [IteratorCollect α m m]
-    [LawfulMonad m] [LawfulMonad n] [LawfulIteratorCollect α m m]
+    [MonadLiftT m (ULiftT n)] [Finite α m]
+    [LawfulMonad m] [LawfulMonad n]
     [LawfulMonadLiftT m (ULiftT n)] :
     (it.uLift n).toArray =
       (fun l => l.down.map ULift.up) <$> (monadLift it.toArray : ULiftT n _).run := by
